dimsum/iris/expr2.v
@@ -25,9 +25,28 @@ Global Arguments mtrans {_ _} _.
 Global Arguments mexpr_rel {_ _} _ _ _.
 Global Arguments mstate_interp {_ _} _ _.
 
+Definition sim_gen_mapsto_state `{!dimsumGS Σ} {EV} (ts : tgt_src) (m : mod_trans EV)
+  Π (H_s : (m_state m) → iProp Σ) : iProp Σ :=
+  ∀ σ, H_s σ -∗ σ ≈{ts, m}≈> Π.
+
+Notation "Pσ '⇒{' ts , m } Π " := (sim_gen_mapsto_state ts m Π Pσ)
+  (at level 20, only parsing) : bi_scope.
+
+Notation "Pσ '⇒{' ts '}' Π " := (sim_gen_mapsto_state ts _ Π Pσ)
+  (at level 20, format "Pσ '⇒{' ts '}'  Π ") : bi_scope.
+Notation "Pσ '⇒{' m '}ₜ' Π " := (sim_gen_mapsto_state Tgt m Π Pσ)
+  (at level 20, only parsing) : bi_scope.
+Notation "Pσ '⇒ₜ' Π" := (sim_gen_mapsto_state Tgt _ Π Pσ)
+  (at level 20, format "Pσ '⇒ₜ' Π ") : bi_scope.
+
+Notation "Pσ '⇒{' m '}ₛ' Π " := (sim_gen_mapsto_state Src m Π Pσ)
+  (at level 20, only parsing) : bi_scope.
+Notation "Pσ '⇒ₛ' Π " := (sim_gen_mapsto_state Src _  Π Pσ)
+  (at level 20, format "Pσ '⇒ₛ' Π ") : bi_scope.
+
 Definition switch `{!dimsumGS Σ} {S EV} (Π : option EV → S → iProp Σ)
-  (K : option EV → S → (tgt_src → ∀ EV2, ∀ m : mod_trans EV2, _ → iProp Σ) → iProp Σ) : iProp Σ :=
-  (∀ κ σ, K κ σ (λ ts' EV2 m' PΠ', ∀ σ' Π', PΠ' σ' Π' -∗ σ' ≈{ ts', m' }≈> Π') -∗  Π κ σ).
+  (K : option EV → S → (tgt_src → ∀ EV2, ∀ m : mod_trans EV2, ∀ Π', _ → iProp Σ) → iProp Σ) : iProp Σ :=
+  (∀ κ σ, K κ σ (λ ts' EV2 m' Π' Pσ', Pσ' ⇒{ts', m'} Π') -∗  Π κ σ).
 
 (* Lemma switch_mono `{!dimsumGS Σ} {S EV} (Π : option EV → S → iProp Σ) K1 K2 : *)
 (*   switch Π K1 -∗ *)
@@ -43,7 +62,7 @@ Definition switch_id `{!dimsumGS Σ} {EV} (ts : tgt_src) (m : mod_trans EV)
   (Π : option EV → m.(m_state) → iProp Σ)
   (κ : option EV) (σ : m.(m_state)) (C : m.(m_state) → iProp Σ) : iProp Σ :=
   switch Π ({{ κs σs POST, ⌜κs = κ⌝ ∗ ⌜σs = σ⌝ ∗
-  POST ts _ m ({{ σ' Πs, ⌜Πs = Π⌝ ∗ C σ'}})}})%I.
+  POST ts _ m Π ({{ σ', C σ'}})}})%I.
 
 Lemma switch_id_mono `{!dimsumGS Σ} {EV} ts (m : mod_trans EV)
   (Π : option EV → m.(m_state) → iProp Σ) κ σ C1 C2 :
@@ -52,7 +71,7 @@ Lemma switch_id_mono `{!dimsumGS Σ} {EV} ts (m : mod_trans EV)
   switch_id ts m Π κ σ C2.
 Proof.
   iIntros "Hs Hmono" (??) "[% [% HC2]]". iApply "Hs".
-  iSplit!. iIntros (??) "[% ?]". iApply "HC2". iSplit!.
+  iSplit!. iIntros (?) "? /=". iApply "HC2". iSplit!.
   by iApply "Hmono".
 Qed.
 
@@ -61,25 +80,25 @@ Qed.
 Definition switch_external `{!dimsumGS Σ} {S EV} (Π : option EV → S → iProp Σ)
   (K : _) : iProp Σ :=
   switch Π ({{ κ σ POST,
-    K κ σ ({{ m2 σ2 K2,
-  POST Src _ m2 ({{ σ_s Π_s,
+    K κ σ ({{ m2 σ2 Π2 K2,
+  POST Src _ m2 Π2 ({{ σ_s,
     ⌜σ_s = σ2⌝ ∗
-  switch Π_s ({{ κ' σ_s2 POST,
+  switch Π2 ({{ κ' σ_s2 POST,
     ⌜κ' = κ⌝ ∗
-  POST Src _ _ ({{ σ_s2' Π',
-    ⌜σ_s2' = σ_s2⌝ ∗ K2 σ_s2 Π'}})}})}})}})}})%I.
+  POST Src _ m2 Π2 ({{ σ_s2',
+    ⌜σ_s2' = σ_s2⌝ ∗ K2 σ_s2}})}})}})}})}})%I.
 
 (* Switching to a linked module *)
 Definition switch_link `{!dimsumGS Σ} {S EV} (ts : tgt_src) (Π : option (io_event EV) → S → iProp Σ)
   (K : _) : iProp Σ :=
   switch Π ({{ κ σ0 POST,
-    K σ0 ({{ e m2 σ2 K2, ⌜κ = Some (Outgoing, e)⌝ ∗
-  POST ts _ m2 ({{ σi Πi,
+    K σ0 ({{ e m2 σ2 Π2 K2, ⌜κ = Some (Outgoing, e)⌝ ∗
+  POST ts _ m2 Π2 ({{ σi,
     ⌜σi = σ2⌝ ∗
-  switch Πi ({{ κ' σ POST,
+  switch Π2 ({{ κ' σ POST,
     ∃ e', ⌜κ' = Some (Incoming, e')⌝ ∗
-  POST ts _ m2 ({{ σr Πr,
-    ⌜σr = σ⌝ ∗ ⌜e' = e⌝ ∗ K2 σ Πr}})}})}})}})}})%I.
+  POST ts _ m2 Π2 ({{ σr,
+    ⌜σr = σ⌝ ∗ ⌜e' = e⌝ ∗ K2 σ}})}})}})}})}})%I.
 
 
 (** * [sim_gen_expr] *)
@@ -103,7 +122,7 @@ Section sim_gen_expr.
   Proof.
     move => ?? Hsim ?? -> ?? HΦ. rewrite /sim_gen_expr_pre.
     repeat (f_equiv || eapply Hsim || eapply HΦ || reflexivity).
-    move => ?? -> ?? ->. unfold switch_id, curly_lambda2, curly_lambda3, switch.
+    move => ?? -> ?? ->. unfold switch_id, curly_lambda2, curly_lambda3, switch, sim_gen_mapsto_state => /=.
     repeat (f_equiv || eapply Hsim || eapply HΦ || reflexivity).
   Qed.
 
@@ -313,9 +332,9 @@ Section sim_gen_expr.
     iApply sim_gen_bind. iApply (sim_gen_wand with "Hsim").
     iIntros (??) "[[% [% [% [??]]]]|Hsim]".
     - iRight. iSplit!. iApply ("HΦ" with "[$] [//] [$]").
-    - iLeft. iApply "Hsim". iSplit!. iIntros (??) "[% [% [% [? HF]]]]". subst.
+    - iLeft. iApply "Hsim". iSplit!. iIntros (?) "[% [% [? HF]]]".
       iApply ("HF" with "[//] [$] [$]").
-Qed.
+  Qed.
 
   Lemma sim_gen_expr_ctx e Π Φ :
     (ord_later_ctx -∗ WP{ts} e @ Π {{ Φ }}) -∗
