dimsum_examples/iris/memmove.v
@@ -4,23 +4,138 @@ Set Default Proof Using "Type".
 
 Local Open Scope Z_scope.
 
+(* TODO - Is this a more general notion we want to factor out somewhere? *)
+Definition splittable {Σ A B} (P : A → iProp Σ) (PL : B → iProp Σ) : iProp Σ :=
+  ∀ a,
+  P a -∗
+  ∃ b, PL b ∗ (PL b -∗ P a).
+
+Section locle.
+  Context `{!dimsumGS Σ} `{!recGS Σ}.
+
+  Definition locle_hoare (P: iProp Σ) ts Π : iProp Σ :=
+    rec_hoare ts Π "locle"
+      (λ es RET, ∃ l1 l2, ⌜es = [Val (ValLoc l1); Val $ ValLoc l2]⌝ ∗ P ∗ RET (l1, l2))%I
+      (λ '(l1, l2) ret, ∃ b, P ∗ ⌜ret = ValBool b⌝ ∗
+                         ⌜l1.1 = l2.1 → b = bool_decide (l1.2 ≤ l2.2)⌝)%I.
+
+  Lemma sim_locle_spec `{!specGS} Π Φ :
+    switch Π ({{ κ σ1 POST,
+      ∃ f es h, ⌜κ = Some (Incoming, ERCall f es h)⌝ ∗
+    POST Tgt _ _ Π ({{ σ',
+      ∃ l1 l2, ⌜σ' = σ1⌝ ∗ ⌜f = "locle"⌝ ∗ ⌜es = [ValLoc l1; ValLoc l2]⌝ ∗
+    switch Π ({{ κ σ POST,
+      ∃ b, ⌜l1.1 = l2.1 → b = bool_decide (l1.2 ≤ l2.2)⌝ ∗
+      ⌜κ = (Some (Outgoing, ERReturn (ValBool b) h))⌝ ∗
+    POST Tgt _ _ Π ({{σ',
+      ⌜σ' = σ⌝ ∗ TGT locle_spec @ Π {{ Φ }}}})}})}})}}) -∗
+    TGT locle_spec @ Π {{ Φ }}.
+  Proof.
+    iIntros "Hs".
+    rewrite {2}/locle_spec unfold_forever /TReceive bind_bind -/locle_spec bind_bind.
+    iApply (sim_tgt_TExist with "[-]"). iIntros ([[??]?]) "!>".
+    rewrite bind_bind. setoid_rewrite bind_ret_l.
+    iApply (sim_gen_TVis with "[-]").
+    iIntros (?) "Hγ !> %% [-> [-> HΠ]]".
+    iApply "Hs". iSplit!. iIntros (?) "(% & % & -> & -> & -> & HC)".
+    iApply "HΠ". iFrame. rewrite bind_bind.
+    iApply (sim_tgt_TAssume with "[-]"); [done|iModIntro]. rewrite bind_bind.
+    iApply (sim_tgt_TAll with "[-]"). iModIntro. rewrite bind_bind.
+    iApply (sim_tgt_TAll with "[-]"). iModIntro. rewrite bind_bind.
+    iApply (sim_tgt_TAssume with "[-]"); [done|iModIntro]. rewrite bind_bind.
+    iApply (sim_tgt_TExist with "[-]"). iIntros (b) "!>". rewrite bind_bind.
+    iApply (sim_tgt_TAssert with "[-]"). iIntros (?) "!>".
+    iApply (sim_gen_TVis with "[-]"). iIntros ([]) "? !>".
+    iIntros (??) "[-> [-> HΠ]]".
+    iApply "HC". iSplit!.
+    iIntros (?) "[-> ?]".
+    iApply "HΠ" => /=. by iFrame.
+  Qed.
+
+  (* The following is not strong enough. Ideally we would write a
+  version where we directly pass a function to K, but this would
+  require a proof that K is monotonic. *)
+  (* Lemma switch_to_id {EV} ts m (Π : option EV → m.(m_state) → iProp Σ) κ σ K C : *)
+  (*   switch Π K -∗ *)
+  (*   (∀ X, (∀ Y, (∀ σ Π', Y σ Π' -∗ ⌜Π' = Π⌝ ∗ C σ) -∗ X ts m Y) -∗ K κ σ X) -∗ *)
+  (*   switch_id ts m Π κ σ C. *)
+  (* Proof. *)
+  (*   iIntros "Hs Hmono" (??) "[-> [-> HC]]". *)
+  (*   iApply "Hs". iApply "Hmono". iIntros (?) "Hmono". *)
+  (*   iIntros (??) "?". iApply "HC". by iApply "Hmono". *)
+  (* Qed. *)
+
+  Lemma sim_locle fns Π_l Π_r (PL : m_state (spec_trans rec_event ()) → iProp Σ) σi :
+    rec_fn_auth fns -∗
+    "locle" ↪ None -∗
+    PL σi -∗
+    ⌜σi.1 ≡ locle_spec⌝ -∗
+    □ switch_link Tgt Π_l ({{σ_l POST,
+      ∃ vs h σg, PL σg ∗
+      POST (ERCall "locle" vs h) (spec_trans _ _) σg Π_r ({{_,
+      switch_link Tgt Π_r ({{σ_r POST,
+        ∃ v h',
+      POST (ERReturn v h') _ σ_l Π_l ({{_,
+        PL σ_r}})}})}})}}) -∗
+    |==> ∃ P, P ∗ □ locle_hoare P Tgt Π_l ∗ □ splittable (λ _ : unit, P) PL.
+  Proof.
+    iIntros "#? #? HPL % #HC".
+    iMod (mstate_var_alloc ()) as (γ) "Hγ".
+    iMod (mstate_var_split γ () with "[$]") as "[Hγ Hγ']".
+    pose (HS := SpecGS γ).
+
+    set P := (∃ σ Φg, PL σ ∗ spec_state () ∗
+                      ({{σ', ⌜σ' = σ⌝ ∗ TGT locle_spec @ Π_r {{Φg}}}}) ⇒ₜ Π_r)%I.
+
+    iExists P.
+    iModIntro. iSplit!.
+    - iExists _, (λ e, sim_post Tgt () Π_r e).
+      iFrame.
+      iIntros ([? []]) "[<- H]".
+      iApply (sim_gen_expr_intro with "[Hγ]") => //=.
+    - iIntros "!> %% (% & % & -> & (% & % & ? & ? & Hg) & HΦ)".
+      iApply (sim_tgt_rec_Call_external with "[$]").
+      iIntros (???) "#??!> %% [-> [-> HΠl]]".
+      iApply "HC". iFrame. iSplit!.
+      iIntros (?) "[-> HC']".
+      iApply "Hg". iSplit!.
+      iApply sim_locle_spec.
+      iIntros (??) "(% & % & % & -> & Hg)".
+      iApply "HC'". iSplit!.
+      iIntros (?) "[% [% HC']]". simplify_eq.
+      iApply "Hg". iSplit!.
+      iIntros (??) "[% [% [-> HΠr]]]".
+      iApply "HC'". iSplit!.
+      iIntros (?) "[-> HC']".
+      iApply sim_tgt_rec_Waiting_all_raw.
+      iIntros (?) "!>". iApply "HC'". iSplit!. iIntros (?) "[-> [-> HPL]]".
+      iApply "HΠl". iSplit!. iFrame.
+      iApply "HΦ". iFrame. iSplit!.
+    - iIntros "!> % (% & % & ? & ?)".
+      iFrame.
+      iIntros "HPL".
+      iFrame.
+  Qed.
+End locle.
+
 Section memmove.
   Context `{!dimsumGS Σ} `{!recGS Σ}.
 
   Lemma sim_memcpy Π :
     "memcpy" ↪ Some memcpy_rec -∗
-    rec_fn_spec_hoare Tgt Π "memcpy" (λ es POST,
-      ∃ d s n o d' s' hvss hvsd, ⌜es = [Val $ ValLoc d; Val $ ValLoc s; Val $ ValNum n; Val $ ValNum o]⌝ ∗
-      ⌜n = Z.of_nat (length hvss)⌝ ∗
-      ⌜length hvss = length hvsd⌝ ∗
-      ⌜o = 1 ∨ o = -1⌝ ∗
-      ⌜d' = (if bool_decide (o = 1) then d else d +ₗ (- n + 1))⌝ ∗
-      ⌜s' = (if bool_decide (o = 1) then s else s +ₗ (- n + 1))⌝ ∗
-      ⌜(if bool_decide (o = 1) then d.1 = s.1 → d.2 ≤ s.2 else d.1 = s.1 → s.2 ≤ d.2)⌝ ∗
-      ([∗ map] l↦v∈array s' hvss ∪ array d' hvsd, l ↦ v) ∗
-      (POST (λ v, ⌜v = 0⌝ ∗ ([∗ map] l↦v∈array d' hvss ∪ array s' hvss, l ↦ v)))).
+    rec_hoare Tgt Π "memcpy"
+      (λ es RET, ∃ d s n o d' s' hvss hvsd,
+        ⌜es = [Val $ ValLoc d; Val $ ValLoc s; Val $ ValNum n; Val $ ValNum o]⌝ ∗
+        ⌜n = Z.of_nat (length hvss)⌝ ∗
+        ⌜length hvss = length hvsd⌝ ∗
+        ⌜o = 1 ∨ o = -1⌝ ∗
+        ⌜d' = (if bool_decide (o = 1) then d else d +ₗ (- n + 1))⌝ ∗
+        ⌜s' = (if bool_decide (o = 1) then s else s +ₗ (- n + 1))⌝ ∗
+        ⌜(if bool_decide (o = 1) then d.1 = s.1 → d.2 ≤ s.2 else d.1 = s.1 → s.2 ≤ d.2)⌝ ∗
+        ([∗ map] l↦v∈array s' hvss ∪ array d' hvsd, l ↦ v) ∗ RET (s', d', hvss))
+      (λ '(s, d, hvss) v, ⌜v = 0⌝ ∗ ([∗ map] l↦v∈array d hvss ∪ array s hvss, l ↦ v)).
   Proof.
-    iIntros "#Hf". iApply rec_fn_spec_hoare_ctx. iIntros "#?".
+    iIntros "#Hf". simpl. iApply rec_hoare_ctx. iIntros "#?".
     iApply ord_loeb; [done|]. iIntros "!> #IH". iIntros (es Φ) "HΦ".
     iDestruct "HΦ" as (d s n o d' s' hvss hvsd ? Hn Hlen Ho Hd' Hs' Hle) "[Hm HΦ]"; simplify_eq/=.
     iApply (sim_tgt_rec_Call_internal with "Hf"); [done|]. iModIntro => /=.
@@ -152,28 +267,25 @@ Section memmove.
         done.
   Qed.
 
-  Definition locle_fn_spec (es : list expr) (POST : (val → iProp Σ) → iProp Σ) : iProp Σ :=
-      ∃ l1 l2, ⌜es = [Val (ValLoc l1); Val $ ValLoc l2]⌝ ∗
-       POST (λ v, ∃ b, ⌜v = ValBool b⌝ ∗ ⌜l1.1 = l2.1 → b = bool_decide (l1.2 ≤ l2.2)⌝).
-
-  Lemma sim_memmove Π :
+  Lemma sim_memmove Π P :
     "memmove" ↪ Some memmove_rec -∗
     "memcpy" ↪ Some memcpy_rec -∗
-    □ rec_fn_spec_hoare Tgt Π "locle" locle_fn_spec -∗
-    rec_fn_spec_hoare Tgt Π "memmove" (λ es POST,
-      ∃ hvss hvsd d s n, ⌜es = [Val (ValLoc d); Val $ ValLoc s; Val $ ValNum n]⌝ ∗
+    □ locle_hoare P Tgt Π -∗
+    rec_hoare Tgt Π "memmove"
+      (λ es RET, ∃ hvss hvsd d s n,
+        ⌜es = [Val (ValLoc d); Val $ ValLoc s; Val $ ValNum n]⌝ ∗
         ⌜n = Z.of_nat (length hvss)⌝ ∗
         ⌜length hvss = length hvsd⌝ ∗
-        ([∗ map] l↦v∈array s hvss ∪ array d hvsd, l ↦ v) ∗
-        (POST (λ v, ⌜v = 0⌝ ∗ ([∗ map] l↦v∈array d hvss ∪ array s hvss, l ↦ v)))).
+        ([∗ map] l↦v∈array s hvss ∪ array d hvsd, l ↦ v) ∗ P ∗ RET (d,s,hvss))%I
+      (λ '(d,s,hvss) v, P ∗ ⌜v = 0⌝ ∗ ([∗ map] l↦v∈array d hvss ∪ array s hvss, l ↦ v))%I.
   Proof.
     iIntros "#Hmemmove #Hmemcpy #Hlocle". iIntros (es Φ) "HΦ".
-    iDestruct "HΦ" as (hvss hvsd d s n -> -> ?) "[Hs HΦ]".
+    iDestruct "HΦ" as (hvss hvsd d s n -> -> ?) "[Hs [? HΦ]]".
     iApply (sim_gen_expr_bind _ []).
     iApply (sim_tgt_rec_Call_internal with "Hmemmove"); [done|]. iModIntro => /=.
     iApply sim_tgt_rec_AllocA; [econs|] => /=. iIntros (?) "?". destruct ls => //. iModIntro.
     iApply (sim_gen_expr_bind _ [IfCtx _ _] with "[-]") => /=.
-    iApply "Hlocle". iExists _, _. iSplit!. iIntros (? [b [-> Hb]]) => /=.
+    iApply "Hlocle". iFrame. iSplit!. iIntros (?) "[%b [? [-> %Hb]]]" => /=.
     iApply sim_tgt_rec_If. iModIntro => /=. destruct b.
     - iApply (sim_memcpy with "[//]"). iFrame. iSplit!. { case_bool_decide; naive_solver. }
       iIntros (?) "[-> ?]". iSplit!. iApply sim_gen_expr_stop. iApply ("HΦ" with "[-]"). by iFrame.
@@ -198,127 +310,64 @@ Section memmove.
       iIntros (?) "[-> ?]". iSplit!. iApply sim_gen_expr_stop. iApply ("HΦ" with "[-]"). by iFrame.
   Qed.
 
+  (* NOTE - REVIEW: We now have fixed Π, but I think it's actually easier to write the lemma without switch_id *)
   (* This spec is tricky to use since one needs to pick one Π upfront *)
-  Lemma sim_locle_spec `{!specGS} Π Φ :
-    (∀ f vs h σ, switch_id Tgt _ Π (Some (Incoming, ERCall f vs h)) σ (λ σ', ∃ l1 l2, ⌜σ' = σ⌝ ∗
-      ⌜f = "locle"⌝ ∗ ⌜vs = [ValLoc l1; ValLoc l2]⌝ ∗ (∀ b,
-        ⌜l1.1 = l2.1 → b = bool_decide (l1.2 ≤ l2.2)⌝ -∗ ∀ σ,
-          switch_id Tgt _ Π (Some (Outgoing, ERReturn (ValBool b) h)) σ (λ σ', ⌜σ' = σ⌝ ∗
-            TGT locle_spec @ Π {{ Φ }})))) -∗
-    TGT locle_spec @ Π {{ Φ }}.
-  Proof.
-    iDestruct 1 as "HC". unfold locle_spec at 2. rewrite unfold_forever -/locle_spec.
-    rewrite /TReceive bind_bind bind_bind.
-    iApply (sim_tgt_TExist with "[-]"). iIntros ([[??]?]) "!>".
-    rewrite bind_bind. setoid_rewrite bind_ret_l.
-    iApply (sim_gen_TVis with "[-]"). iIntros ([]) "? !>".
-    iApply (switch_id_mono with "HC"). iIntros (?). iDestruct 1 as (l1 l2 -> -> ->) "HC" => /=. iFrame.
-    rewrite bind_bind. iApply (sim_tgt_TAssume with "[-]"); [done|]. iIntros "!>".
-    rewrite bind_bind. iApply (sim_tgt_TAll with "[-]"). iIntros "!>".
-    rewrite bind_bind. iApply (sim_tgt_TAll with "[-]"). iIntros "!>".
-    rewrite bind_bind. iApply (sim_tgt_TAssume with "[-]"); [done|]. iIntros "!>".
-    rewrite bind_bind. iApply (sim_tgt_TExist with "[-]"). iIntros (b) "!>".
-    rewrite bind_bind. iApply (sim_tgt_TAssert with "[-]"). iIntros (?) "!>".
-    iApply (sim_gen_TVis with "[-]"). iIntros ([]) "? !>".
-    iApply (switch_id_mono with "[HC]"). { iApply ("HC" with "[//]"). }
-    simpl. iIntros (?). iDestruct 1 as (->) "HC". iFrame.
-  Qed.
-
-  (* The following is not strong enough. Ideally we would write a
-  version where we directly pass a function to K, but this would
-  require a proof that K is monotonic. *)
-  (* Lemma switch_to_id {EV} ts m (Π : option EV → m.(m_state) → iProp Σ) κ σ K C : *)
-  (*   switch Π K -∗ *)
-  (*   (∀ X, (∀ Y, (∀ σ Π', Y σ Π' -∗ ⌜Π' = Π⌝ ∗ C σ) -∗ X ts m Y) -∗ K κ σ X) -∗ *)
-  (*   switch_id ts m Π κ σ C. *)
+  (* Lemma sim_locle_spec' `{!specGS} Π Φ : *)
+  (*   (∀ f vs h σ, switch_id Tgt _ Π (Some (Incoming, ERCall f vs h)) σ (λ σ', ∃ l1 l2, ⌜σ' = σ⌝ ∗ *)
+  (*     ⌜f = "locle"⌝ ∗ ⌜vs = [ValLoc l1; ValLoc l2]⌝ ∗ (∀ b, *)
+  (*       ⌜l1.1 = l2.1 → b = bool_decide (l1.2 ≤ l2.2)⌝ -∗ ∀ σ, *)
+  (*         switch_id Tgt _ Π (Some (Outgoing, ERReturn (ValBool b) h)) σ (λ σ', ⌜σ' = σ⌝ ∗ *)
+  (*           TGT locle_spec @ Π {{ Φ }})))) -∗ *)
+  (*   TGT locle_spec @ Π {{ Φ }}. *)
   (* Proof. *)
-  (*   iIntros "Hs Hmono" (??) "[-> [-> HC]]". *)
-  (*   iApply "Hs". iApply "Hmono". iIntros (?) "Hmono". *)
-  (*   iIntros (??) "?". iApply "HC". by iApply "Hmono". *)
+  (*   iDestruct 1 as "HC". unfold locle_spec at 2. rewrite unfold_forever -/locle_spec. *)
+  (*   rewrite /TReceive bind_bind bind_bind. *)
+  (*   iApply (sim_tgt_TExist with "[-]"). iIntros ([[??]?]) "!>". *)
+  (*   rewrite bind_bind. setoid_rewrite bind_ret_l. *)
+  (*   iApply (sim_gen_TVis with "[-]"). iIntros ([]) "? !>". *)
+  (*   iApply (switch_id_mono with "HC"). iIntros (?). iDestruct 1 as (l1 l2 -> -> ->) "HC" => /=. iFrame. *)
+  (*   rewrite bind_bind. iApply (sim_tgt_TAssume with "[-]"); [done|]. iIntros "!>". *)
+  (*   rewrite bind_bind. iApply (sim_tgt_TAll with "[-]"). iIntros "!>". *)
+  (*   rewrite bind_bind. iApply (sim_tgt_TAll with "[-]"). iIntros "!>". *)
+  (*   rewrite bind_bind. iApply (sim_tgt_TAssume with "[-]"); [done|]. iIntros "!>". *)
+  (*   rewrite bind_bind. iApply (sim_tgt_TExist with "[-]"). iIntros (b) "!>". *)
+  (*   rewrite bind_bind. iApply (sim_tgt_TAssert with "[-]"). iIntros (?) "!>". *)
+  (*   iApply (sim_gen_TVis with "[-]"). iIntros ([]) "? !>". *)
+  (*   iApply (switch_id_mono with "[HC]"). { iApply ("HC" with "[//]"). } *)
+  (*   simpl. iIntros (?). iDestruct 1 as (->) "HC". iFrame. *)
   (* Qed. *)
 
-  (* This spec does not require one to pick Π upfront *)
-  Lemma sim_locle_spec2 `{!specGS} Π Φ :
-    switch Π ({{ κ σ POST,
-      ∃ f vs h, ⌜κ = Some (Incoming, ERCall f vs h)⌝ ∗
-    POST Tgt _ (spec_trans _ unit) ({{ σ' Π',
-      ∃ l1 l2, ⌜σ' = σ⌝ ∗ ⌜f = "locle"⌝ ∗ ⌜vs = [ValLoc l1; ValLoc l2]⌝ ∗
-    switch Π' ({{ κ σ POST,
-      ∃ b, ⌜l1.1 = l2.1 → b = bool_decide (l1.2 ≤ l2.2)⌝ ∗
-      ⌜κ = (Some (Outgoing, ERReturn (ValBool b) h))⌝ ∗ ⌜σ = (locle_spec, tt)⌝ ∗
-      spec_state ()
-      }})}})}}) -∗
-    TGT locle_spec @ Π {{ Φ }}.
-  Proof.
-    iDestruct 1 as "HC". unfold locle_spec at 2. rewrite unfold_forever -/locle_spec.
-    rewrite /TReceive bind_bind bind_bind.
-    iApply (sim_tgt_TExist with "[-]"). iIntros ([[??]?]) "!>".
-    rewrite bind_bind. setoid_rewrite bind_ret_l.
-    iApply (sim_gen_TVis with "[-]"). iIntros ([]) "Hs !>".
-    (* iApply (switch_to_id with "HC"). iIntros (?) "HX". *)
-    iIntros (??) "[% [% _]]". subst.
-    iApply "HC". iSplit!. iIntros (??). iDestruct 1 as (?????) "HC". subst.
-    iApply (sim_gen_expr_intro _ tt with "[Hs]"); simpl; [done..|].
-    rewrite bind_bind. iApply (sim_tgt_TAssume with "[-]"); [done|]. iIntros "!>".
-    rewrite bind_bind. iApply (sim_tgt_TAll with "[-]"). iIntros "!>".
-    rewrite bind_bind. iApply (sim_tgt_TAll with "[-]"). iIntros "!>".
-    rewrite bind_bind. iApply (sim_tgt_TAssume with "[-]"); [done|]. iIntros "!>".
-    rewrite bind_bind. iApply (sim_tgt_TExist with "[-]"). iIntros (b) "!>".
-    rewrite bind_bind. iApply (sim_tgt_TAssert with "[-]"). iIntros (?) "!>".
-    iApply (sim_gen_TVis with "[-]"). iIntros ([]) "? !>".
-    iIntros (??) "[% [% _]]". subst. iApply "HC". iSplit!.
-  Qed.
+End memmove.
 
-  Lemma sim_locle2 fns Π :
-    rec_fn_auth fns -∗
-    "locle" ↪ None -∗
-    switch_link Tgt Π ({{ σ0 POST,
-      ∃ vs h,
-    POST (ERCall "locle" vs h) (spec_trans _ _) (locle_spec, tt) ({{ _ Πr,
-    switch_link Tgt Πr ({{ σ POST,
-      ∃ v h', ⌜σ = (locle_spec, tt)⌝ ∗
-    POST (ERReturn v h') _ σ0 ({{ _ Πx,
-      ⌜Πx = Π⌝}})}})}})}}) -∗
-    rec_fn_spec_hoare Tgt Π "locle" locle_fn_spec.
-  Proof.
-    iIntros "#Hfns #Hf HΠ" (es Φ) "HΦ". iDestruct "HΦ" as (l1 l2 ->) "HΦ".
-    iApply (sim_tgt_rec_Call_external with "[$]"). iIntros (???) "#?? !>".
-    iIntros (??) "[% [% Hσ]]". subst. iApply "HΠ". iSplit!. iIntros (??) "[-> HΠi]".
-    iMod (mstate_var_alloc unit) as (γ) "?".
-    iMod (mstate_var_split γ tt with "[$]") as "[Hγ ?]".
-    pose (Hspec := SpecGS γ).
-    iApply (sim_gen_expr_intro _ tt with "[Hγ]"); simpl; [done..|].
-    iApply sim_locle_spec2 => /=. iIntros (??). iDestruct 1 as (????) "HC". subst.
-    iApply "HΠi". iSplit!. iIntros (??) "[% [% HΠr]]". simplify_eq/=.
-    iApply "HC". iSplit!. iIntros (??). iDestruct 1 as (????) "HC".
-    iApply "HΠr". iSplit!. iIntros (??) "[% HΠf]". simplify_eq.
-    iApply sim_tgt_rec_Waiting_raw.
-    iSplit. { iIntros. iModIntro. iApply "HΠf". iSplit!. iIntros (??) "[% [% ?]]". simplify_eq. }
-    iIntros (???) "!>". iApply "HΠf". iSplit!. iIntros (??[?[??]]). simplify_eq.
-    iApply "Hσ". iSplit!. iFrame. iApply "HΦ". iSplit!.
-  Qed.
+Section main.
+  Context `{!dimsumGS Σ} `{!recGS Σ}.
 
-  Lemma sim_main Π :
+  Lemma sim_main Π P :
     "memmove" ↪ Some memmove_rec -∗
     "memcpy" ↪ Some memcpy_rec -∗
     "main" ↪ Some main_rec -∗
-    □ rec_fn_spec_hoare Tgt Π "locle" locle_fn_spec -∗
-    rec_fn_spec_hoare Tgt Π "main" (λ es POST, ⌜es = []⌝ ∗
-      rec_fn_spec_hoare Tgt Π "print" (λ es POST1, ⌜es = [Val 1]⌝ ∗ POST1 (λ _,
-        rec_fn_spec_hoare Tgt Π "print" (λ es POST2, ⌜es = [Val 2]⌝ ∗ POST2 (λ _, POST (λ v, ⌜v = 0⌝)))))).
+    □ locle_hoare P Tgt Π -∗
+    rec_hoare Tgt Π "main" (λ es RET, ⌜es = []⌝ ∗ P ∗
+      rec_hoare Tgt Π "print"
+        (λ es RET, P ∗ ⌜es = [Val 1]⌝ ∗ RET tt)
+        (λ _ v, rec_hoare Tgt Π "print"
+                  (λ es RET, ⌜es = [Val 2]⌝ ∗ RET tt)
+                  (λ _ _, RET tt)))
+        (λ _ v, ⌜v = 0⌝).
   Proof.
-    iIntros "#? #? #? #?". iIntros (es Φ). iDestruct 1 as (->) "HΦ".
+    iIntros "#? #? #? #?". iIntros (es Φ) "[-> [? HΦ]]".
     iApply sim_tgt_rec_Call_internal. 2: { done. } { done. }
-    iModIntro => /=.
-    iApply sim_tgt_rec_AllocA; [by econs|] => /=. iIntros (?) "Hl".
+    iModIntro.
+    iApply sim_tgt_rec_AllocA; [by econs|]. iIntros (?) "Hl".
     destruct ls as [|l []] => //=. 2: by iDestruct!.
-    have -> : (0%nat + 0) = 0 by []. have -> : (1%nat + 0) = 1 by []. have -> : (2%nat + 0) = 2 by [].
+    have -> : (0%nat + 0) = 0 by [].
+    have -> : (1%nat + 0) = 1 by []. have -> : (2%nat + 0) = 2 by [].
     iDestruct "Hl" as "[[Hl0 [Hl1 [Hl2 _]]] _]". iModIntro.
-    iApply (sim_gen_expr_bind _ [LetECtx _ _] with "[-]") => /=.
-    iApply (sim_gen_expr_bind _ [StoreLCtx _] with "[-]") => /=.
-    iApply sim_tgt_rec_BinOp; [done|]. iModIntro => /=.
+    iApply (sim_gen_expr_bind _ [LetECtx _ _] with "[-]").
+    iApply (sim_gen_expr_bind _ [StoreLCtx _] with "[-]").
+    iApply sim_tgt_rec_BinOp; [done|iModIntro].
     iApply (sim_tgt_rec_Store with "Hl0"). iIntros "Hl0 !>" => /=.
-    iApply sim_tgt_rec_LetE. iIntros "!>" => /=.
+    iApply sim_tgt_rec_LetE. iIntros "!> /=".
     iApply (sim_gen_expr_bind _ [LetECtx _ _] with "[-]") => /=.
     iApply (sim_gen_expr_bind _ [StoreLCtx _] with "[-]") => /=.
     iApply sim_tgt_rec_BinOp; [done|]. iModIntro => /=.
@@ -338,7 +387,9 @@ Section memmove.
       iApply (big_sepM_insert_2 with "[Hl1]"); [done|].
       iApply (big_sepM_insert_2 with "[Hl2]"); [done|].
       done. }
-    iIntros (?) "[-> Hl]" => /=. rewrite !array_cons !array_nil -!insert_union_l !left_id_L.
+    iFrame.
+    iIntros (?) "[? [-> Hl]]" => /=.
+    rewrite !array_cons !array_nil -!insert_union_l !left_id_L.
     rewrite !offset_loc_assoc.
     rewrite (big_sepM_delete _ _ (l +ₗ 1)). 2: { by simplify_map_eq. }
     rewrite delete_insert_delete.
@@ -355,7 +406,7 @@ Section memmove.
     iApply sim_tgt_rec_BinOp; [done|]. iModIntro => /=.
     iApply (sim_tgt_rec_Load with "Hl1"). iIntros "Hl1 !>" => /=.
 
-    iApply "HΦ". iSplit!. iIntros (?) "HΦ".
+    iApply "HΦ". iFrame. iSplit!. iIntros (?) "HΦ".
 
     iApply (sim_tgt_rec_LetE with "[-]"). iIntros "!>" => /=.
     iApply (sim_gen_expr_bind _ [LetECtx _ _] with "[-]") => /=.
@@ -364,267 +415,278 @@ Section memmove.
     iApply sim_tgt_rec_BinOp; [done|]. iModIntro => /=.
     iApply (sim_tgt_rec_Load with "Hl2"). iIntros "Hl2 !>" => /=.
 
-    iApply "HΦ". iSplit!. iIntros (?) "HΦ".
+    iApply "HΦ". iFrame. iSplit!. iIntros (?) "HΦ".
 
     iApply (sim_tgt_rec_LetE with "[-]"). iIntros "!>" => /=.
     iApply sim_gen_expr_stop => /=. iSplit!. iFrame. by iApply "HΦ".
   Qed.
 
+  Definition call_print v : spec rec_event unit unit :=
+    h ← TExist _;
+    '(_,h') ← TCallRet "print" [ValNum v] h;
+    TAssume (h = h').
+  
   Definition main_spec_body : spec rec_event unit void :=
-    h' ← TExist _;
-    TVis (Outgoing, ERCall "print" [ValNum 1] h');;
-    e ← TExist _;
-    TVis (Incoming, e);;
-    TAssume (if e is ERReturn _ h'' then h' = h'' else false);;
-    h' ← TExist _;
-    TVis (Outgoing, ERCall "print" [ValNum 2] h');;
-    e ← TExist _;
-    TVis (Incoming, e);;
-    TAssume (if e is ERReturn _ h'' then h' = h'' else false);;
+    call_print 1;;
+    call_print 2;;
     TUb.
 
-  Lemma sim_main_full Π γσ_s (σ : m_state (spec_trans _ unit)) :
-    "memmove" ↪ Some memmove_rec -∗
-    "memcpy" ↪ Some memcpy_rec -∗
-    "main" ↪ Some main_rec -∗
+  Definition print_ext_hoare `{specGS}
+      (PL : m_state (spec_trans rec_event ()) → iProp Σ) ts Π : iProp Σ :=
+    rec_hoare ts Π "print"
+      (λ es RET, ∃ σ v k, spec_state_name ⤳@{unit} - ∗
+        PL σ ∗ ⌜σ.1 ≡ Spec.bind (call_print v) k⌝ ∗ ⌜es = [Val v]⌝ ∗ RET k)%I
+      (λ k _, ∃ σ_s, PL σ_s ∗ spec_state_name ⤳@{unit} - ∗ ⌜σ_s.1 ≡ k tt⌝)%I.
+
+  Lemma call_print_sim (S : specGS) fns PL Π_t Π_s :
+    rec_fn_auth fns -∗
     "print" ↪ None -∗
-    □ rec_fn_spec_hoare Tgt Π "locle" locle_fn_spec -∗
-    γσ_s ⤳ σ -∗
-    ⌜σ.1 ≡ main_spec_body⌝ -∗
-    rec_fn_spec_hoare Tgt Π "main" (λ es POST,
-      ⌜es = []⌝ ∗
-      □ switch_external Π (λ κ σ POST,
-          ∃ vs h σ_s, ⌜κ = Some (Outgoing, ERCall "print" vs h)⌝ ∗ γσ_s ⤳ σ_s ∗
-        POST (spec_trans _ unit) σ_s (λ _ Π',
-        (* TODO: Some nice abstraction for the following? *)
-          ∃ e,
-        switch Π' (λ κ'' σ_s3 POST,
-          ⌜κ'' = Some (Incoming, e)⌝ ∗
-        POST Src _ _ (λ σ_s3' Π_s'',
-          ⌜σ_s3' = σ_s3⌝ ∗
-        switch Π_s'' (λ κ'' σ'' POST,
-          ∃ v h', ⌜e = ERReturn v h'⌝ ∗ ⌜κ'' = None⌝ ∗
-        POST Tgt _ _ (λ σ' Π',
-          ⌜σ' = σ⌝ ∗ γσ_s ⤳ σ'' ∗
-        switch Π' (λ κ σ POST,
-          ∃ e', ⌜κ = Some (Incoming, e')⌝ ∗
-        POST Tgt _ _ (λ σ' Π',
-          ⌜σ' = σ⌝ ∗ ⌜e = e'⌝ ∗ ⌜Π = Π'⌝)))))))) ∗
-      POST (λ vr, ∃ σ_s, γσ_s ⤳ σ_s ∗ (∀ Π, σ_s ≈{ spec_trans rec_event () }≈>ₛ Π) ∗ ⌜vr = 0⌝)).
+    □ switch_external Π_t ({{κ0 σ_t POST0,
+        ∃ vs h σs, PL σs ∗ ⌜κ0 = Some (Outgoing, ERCall "print" vs h)⌝ ∗
+      POST0 (spec_trans _ ()) σs Π_s ({{σ_s1',
+        ∃ e : rec_ev,
+      switch Π_s ({{ κ3 σ_s2 POST2,
+        ⌜κ3 = Some (Incoming, e)⌝ ∗
+      POST2 Src _ (spec_trans _ ()) Π_s ({{ σ_s2',
+        ⌜σ_s2 = σ_s2'⌝ ∗
+      switch Π_s ({{ κ4 σ_s3 POST3,
+        ∃ v h', ⌜e = ERReturn v h'⌝ ∗ ⌜κ4 = None⌝ ∗
+      POST3 Tgt _ _ Π_t ({{ σ_t1,
+        ⌜σ_t1 = σ_t⌝ ∗
+      switch Π_t ({{ κ5 σ_t2 POST4,
+        ∃ e' : rec_ev, ⌜κ5 = Some (Incoming, e')⌝ ∗
+      POST4 Tgt rec_event rec_trans Π_t ({{ σ_t3,
+        ⌜σ_t3 = σ_t2⌝ ∗ ⌜e = e'⌝ ∗ PL σ_s3
+    }})}})}})}})}})}})}})}}) -∗
+    □ print_ext_hoare PL Tgt Π_t.
   Proof.
+    set γ := spec_state_name.
     set (X := (switch_external _) _).
-    iIntros "#?#?#?#?#? Hσs". iIntros (??). iDestruct 1 as (?) "[#Hs Hend]".
-    iMod (mstate_var_alloc unit) as (γ) "?".
-    iMod (mstate_var_split γ σ.2 with "[$]") as "[Hγ ?]".
-    pose (Hspec := SpecGS γ).
-
-    iApply sim_main; [done..|]. iSplit!.
-
-    iIntros (??). iDestruct 1 as (->) "HΦ".
-    iApply (sim_tgt_rec_Call_external); [done|].
-    iIntros (???) "Hfns' Hh !>". iIntros (??) "[-> [-> Hσ]]".
-    iApply "Hs". iSplit!. iFrame. iSplit!. iIntros (??) "[-> HC]".
+    iIntros "#?#?#HC !> %% (%σ & % & % & ? & ? & % & -> & HΦ)".
+    iMod (mstate_var_split γ σ.2 with "[$]") as "[Hγ Hγ']".
+    iApply (sim_tgt_rec_Call_external with "[$]").
+    iIntros (???) "#?? !>".
+    iIntros (??) "[-> [-> HΠ_t]]".
+    iApply "HC". iFrame. iSplit!.
+    iIntros (?) "[-> HC']".
+    (* TODO *)
     iApply (sim_gen_expr_intro _ tt with "[Hγ] [-]"); simpl; [done..|].
-    unfold main_spec_body.
-    iApply (sim_src_TExist _).
-    iApply sim_gen_TVis. iIntros ([]) "Hγ".
-    iIntros (??) "[-> [-> ?]]".
-    iApply "HC". iSplit!. iIntros (??) "[-> [% HC]]".
-    iApply (sim_gen_expr_intro _ tt with "[Hγ] [-]"); [simpl; done..|].
-    iApply (sim_src_TExist _).
-    iApply sim_gen_TVis. iIntros ([]) "Hγ".
-    iIntros (??) "[-> [-> ?]]".
-    iApply "HC". iSplit!. iIntros (??) "[-> HC]".
-    iApply (sim_gen_expr_intro _ tt with "[Hγ] [-]"); [simpl; done..|].
-    iApply sim_src_TAssume. iIntros (?). case_match => //; simplify_eq/=.
-    iApply sim_gen_expr_None => /=. iIntros (? [] ?) "Hγ".
-    iIntros (??) "[-> [-> ?]]".
-    iApply "HC". iSplit!. iIntros (??) "[-> [? HC]]".
-    iApply sim_tgt_rec_Waiting_raw.
-    iSplit. { iIntros. iModIntro. iApply "HC". iSplit!. iIntros (??) "[% [% %]]". simplify_eq. }
-    iIntros (?? _) "!>". iApply "HC". iSplit!. iIntros (??[?[??]]). simplify_eq/=.
-    iApply "Hσ". iSplit!. iFrame. iApply "HΦ".
-
-    iIntros (??). iDestruct 1 as (->) "HΦ".
-    iApply (sim_tgt_rec_Call_external); [done|].
-    iIntros (???) "Hfns'' Hh !>". iIntros (??) "[-> [-> Hσ]]".
-    iApply "Hs". iSplit!. iFrame. iSplit!. iIntros (??) "[-> HC]".
-    iApply (sim_gen_expr_intro _ tt with "[Hγ] [-]"); simpl; [done..|].
-    unfold main_spec_body.
-    iApply (sim_src_TExist _).
-    iApply sim_gen_TVis. iIntros ([]) "Hγ".
-    iIntros (??) "[-> [-> ?]]".
-    iApply "HC". iSplit!. iIntros (??) "[-> [% HC]]".
-    iApply (sim_gen_expr_intro _ tt with "[Hγ] [-]"); [simpl; done..|].
-    iApply (sim_src_TExist _).
-    iApply sim_gen_TVis. iIntros ([]) "Hγ".
-    iIntros (??) "[-> [-> ?]]".
-    iApply "HC". iSplit!. iIntros (??) "[-> HC]".
-    iApply (sim_gen_expr_intro _ tt with "[Hγ] [-]"); [simpl; done..|].
-    iApply sim_src_TAssume. iIntros (?). case_match => //; simplify_eq/=.
-    iApply sim_gen_expr_None => /=. iIntros (? [] ?) "Hγ".
-    iIntros (??) "[-> [-> ?]]".
-    iApply "HC". iSplit!. iIntros (??) "[-> [? HC]]".
-    iApply sim_tgt_rec_Waiting_raw.
-    iSplit. { iIntros. iModIntro. iApply "HC". iSplit!. iIntros (??) "[% [% %]]". simplify_eq. }
-    iIntros (?? _) "!>". iApply "HC". iSplit!. iIntros (??[?[??]]). simplify_eq/=.
-    iApply "Hσ". iSplit!. iFrame. iApply "HΦ". iIntros (? ->).
-
-    iApply ("Hend" with "[-]"). iFrame. iSplit!. iIntros (?).
-    iApply (sim_gen_expr_intro _ tt with "[Hγ] [-]"); [simpl; done..|].
-    iApply sim_src_TUb_end.
+    rewrite bind_bind.
+    iApply sim_src_TExist. rewrite bind_bind.
+    iApply sim_src_TCallRet.
+    iIntros (??) "(% & % & % & -> & -> & -> & -> & HΠ_s)".
+    iApply "HC'". iSplit!.
+    iIntros (?) "[-> [% HC']]".
+    iApply "HΠ_s". iSplit!. iIntros (??) "[-> HΠ_s]".
+    iApply "HC'". iSplit!. iIntros (?) "[-> HC']".
+    iApply "HΠ_s". iSplit!. iIntros (?? ->).
+    iApply sim_src_TAssume. iIntros "->".
+    iApply sim_gen_expr_None => /=.
+    iIntros (?) "_ % ? %% /= [-> [-> H]]".
+    iApply "HC'". iSplit!.
+    iIntros (?) "/= [-> HC']".
+    iApply sim_tgt_rec_Waiting_all_raw. iIntros (?) "!>".
+    iApply "HC'". iSplit!. iIntros (?) "[-> [<- ?]]" => /=.
+    iApply "HΠ_t". iSplit!. iFrame.
+    iApply "HΦ".
+    iDestruct (mstate_var_merge with "Hγ' [$]") as "[_ ?]".
+    by iFrame.
   Qed.
 
+  Definition main_spec : spec rec_event unit void :=
+    '(f, vs, h) ← TReceive (λ '(f, vs, h), (Incoming, ERCall f vs h));
+    TAssume (f = "main");;
+    TAssume (vs = []);;
+    main_spec_body.
 
-
-  (* (* Writing this spec for main_spec probably does not gain much / if *)
-  (* anything compared to reasoning about the spec module directly *) *)
-  (* Lemma sim_main_spec Π Φ : *)
-  (*   (∃ f vs h, ∀ σ, handle_cont _ Src Π (Some (Incoming, ERCall f vs h)) σ (λ σ', ⌜σ' = σ⌝ ∗ ( *)
-  (*     ⌜f = "main"⌝ -∗ ⌜vs = []⌝ -∗ *)
-  (*     ∀ σ, handle_cont _ Src Π None σ (λ σ', ⌜σ = σ'⌝ ∗ *)
-  (*     (∃ h', ∀ σ, handle_cont _ Src Π (Some (Outgoing, ERCall "print" [ValNum 1] h')) σ (λ σ', ⌜σ' = σ⌝ ∗ *)
-  (*     (∃ e, ∀ σ, handle_cont _ Src Π (Some (Incoming, e)) σ (λ σ', ⌜σ' = σ⌝ ∗ (∀ v', ⌜e = ERReturn v' h'⌝ -∗ *)
-  (*     ∀ σ, handle_cont _ Src Π None σ (λ σ', ⌜σ = σ'⌝ ∗ *)
-  (*     (∃ h', ∀ σ, handle_cont _ Src Π (Some (Outgoing, ERCall "print" [ValNum 2] h')) σ (λ σ', ⌜σ' = σ⌝ ∗ *)
-  (*     (∃ e, ∀ σ, handle_cont _ Src Π (Some (Incoming, e)) σ (λ σ', ⌜σ' = σ⌝ ∗ (∀ v', ⌜e = ERReturn v' h'⌝ -∗ *)
-  (*     ∀ σ, handle_cont _ Src Π None σ (λ σ', ⌜σ = σ'⌝ ∗ True)))))))))))))))) -∗ *)
-  (*   SRC main_spec @ Π {{ Φ }}. *)
-  (* Proof. *)
-  (*   iIntros "HΦ". iDestruct "HΦ" as (f vs h) "HΦ". *)
-  (*   iEval (unfold main_spec). rewrite /TReceive bind_bind. *)
-  (*   iApply (sim_src_TExist (_, _, _)). *)
-  (*   rewrite bind_bind. setoid_rewrite bind_ret_l. *)
-  (*   iApply sim_gen_TVis. iIntros ([]). iApply (handle_cont_mono with "HΦ"). *)
-  (*   iIntros (?) "[-> HΦ]". iSplit; [done|]. *)
-  (*   iApply sim_src_TAssume. iIntros (?). *)
-  (*   iApply sim_src_TAssume. iIntros (?). simplify_eq. *)
-  (*   iDestruct ("HΦ" with "[//] [//]") as "HΦ". *)
-  (*   iApply sim_gen_expr_None => /=. iIntros (? [] ??). iApply (handle_cont_mono with "HΦ"). *)
-  (*   iIntros (?) "[-> [% HΦ]]". iExists _. iSplit; [done|]. iSplit!. *)
-  (*   iApply sim_src_TExist. iApply sim_gen_TVis. iIntros ([]). iApply (handle_cont_mono with "HΦ"). *)
-  (*   iIntros (?) "[-> [% HΦ]]". iSplit; [done|]. *)
-  (*   iApply sim_src_TExist. iApply sim_gen_TVis. iIntros ([]). iApply (handle_cont_mono with "HΦ"). *)
-  (*   iIntros (?) "[-> HΦ]". iSplit; [done|]. *)
-  (*   iApply sim_src_TAssume. iIntros (?). case_match => //; simplify_eq. *)
-  (*   iDestruct ("HΦ" with "[//]") as "HΦ". *)
-  (*   iApply sim_gen_expr_None => /=. iIntros (? [] ??). iApply (handle_cont_mono with "HΦ"). *)
-  (*   iIntros (?) "[-> [% HΦ]]". iExists _. iSplit; [done|]. iSplit!. *)
-  (*   iApply sim_src_TExist. iApply sim_gen_TVis. iIntros ([]). iApply (handle_cont_mono with "HΦ"). *)
-  (*   iIntros (?) "[-> [% HΦ]]". iSplit; [done|]. *)
-  (*   iApply sim_src_TExist. iApply sim_gen_TVis. iIntros ([]). iApply (handle_cont_mono with "HΦ"). *)
-  (*   iIntros (?) "[-> HΦ]". iSplit; [done|]. *)
-  (*   iApply sim_src_TAssume. iIntros (?). case_match => //; simplify_eq. *)
-  (*   iDestruct ("HΦ" with "[//]") as "HΦ". *)
-  (*   iApply sim_gen_expr_None => /=. iIntros (? [] ??). iApply (handle_cont_mono with "HΦ"). *)
-  (*   iIntros (?) "[-> HΦ]". iExists _. iSplit; [done|]. iSplit!. *)
-  (*   iApply sim_src_TUb_end. *)
-  (* Qed. *)
-End memmove.
-
-Section memmove.
-  Context `{!dimsumGS Σ} `{!recGS Σ}.
-
-  Let m_t := rec_link_trans {["main"; "memmove"; "memcpy"]} {["locle"]} rec_trans (spec_trans rec_event ()).
+  Let m_t := rec_link_trans {["main"; "memmove"; "memcpy"]} {["locle"]}
+               rec_trans (spec_trans rec_event ()).
 
   Lemma memmove_sim :
     rec_state_interp (rec_init (main_prog ∪ memmove_prog ∪ memcpy_prog)) None -∗
     (MLFRun None, [], rec_init (main_prog ∪ memmove_prog ∪ memcpy_prog), (locle_spec, ())) ⪯{m_t,
-      spec_trans rec_event ()} (main_spec, ()).
+      spec_trans rec_event unit} (main_spec, tt).
   Proof.
-    iIntros "[#Hfns Hh] /=".
-    iMod (mstate_var_alloc (m_state (spec_trans rec_event ()))) as (γσ_s) "Hγσ_s".
+    iIntros "[#Hfns ?] /=".
+    (* Ghost variable for source, target, and event *)
+    iMod (mstate_var_alloc (m_state (spec_trans rec_event unit))) as (γσ_s) "Hγσ_s".
     iMod (mstate_var_alloc (m_state m_t)) as (γσ_t) "Hγσ_t".
     iMod (mstate_var_alloc (option rec_event)) as (γκ) "Hγκ".
-    (* iMod (mstate_var_alloc (list seq_product_case)) as (γs) "Hγs". *)
-    (* iMod (mstate_var_alloc (m_state (spec_trans rec_event ()))) as (γσ_locle) "Hγσ_locle". *)
-    iMod (mstate_var_alloc unit) as (γs) "?".
-    iMod (mstate_var_split γs tt with "[$]") as "[Hγs ?]".
-    pose (Hspec := SpecGS γs).
+    (* Source's state *)
+    iMod (mstate_var_alloc unit) as (γs_s) "?".
+    iMod (mstate_var_split γs_s tt with "[$]") as "[Hγs_s ?]".
+    pose (Hspec := SpecGS γs_s).
 
     iApply (sim_tgt_constP_intro γσ_t γσ_s γκ with "Hγσ_t Hγσ_s Hγκ [-]"). iIntros "Hγσ_s".
     iApply (sim_tgt_link_None with "[-]").
     iIntros "!>" (??????). destruct!/=. case_match; destruct!/=.
     iApply (sim_tgt_constP_elim γσ_t γσ_s γκ with "[Hγσ_s] [-]"); [done..|].
     iIntros "Hγσ_s Hγσ_t Hγκ".
-    iApply (sim_gen_expr_intro _ tt with "[Hγs] [-]"); [simpl; done..|].
-    iEval (unfold main_spec). rewrite /TReceive bind_bind.
+    iApply (sim_gen_expr_intro _ tt with "[Hγs_s] [-]"); [simpl; done..|].
+    iEval (rewrite /main_spec /TReceive bind_bind).
     iApply (sim_src_TExist (_, _, _)).
     rewrite bind_bind. setoid_rewrite bind_ret_l.
-    iApply sim_gen_TVis. iIntros ([]) "Hγs". iIntros (??) "[-> [-> _]]".
+    iApply sim_gen_TVis. iIntros ([]) "Hγs". iIntros (??) "[-> [-> HΠ_s]]".
     iApply (sim_src_constP_next with "[Hγσ_t] [Hγκ] [Hγσ_s] [%] [-]"); [done..|].
     iIntros "Hγσ_s". iApply sim_gen_stop.
     iApply (sim_tgt_constP_elim γσ_t γσ_s γκ with "[Hγσ_s] [-]"); [done..|].
     iIntros "Hγσ_s Hγσ_t Hγκ".
-    iApply (sim_gen_expr_intro _ tt with "[Hγs] [-]"); [simpl; done..|].
-    iApply sim_src_TAssume. iIntros (?).
-    iApply sim_src_TAssume. iIntros (?). simplify_eq.
+    iApply "HΠ_s". iFrame.
+    iApply sim_src_TAssume. iIntros (->).
+    iApply sim_src_TAssume. iIntros (->).
     iApply sim_gen_expr_None => /=. iIntros (? [] ?) "Hγs".
+    (* TODO - Here for external call *)
     iIntros (??) "[-> [-> _]]".
 
     rewrite bool_decide_true; [|done].
     iApply (sim_src_constP_next with "[Hγσ_t] [Hγκ] [Hγσ_s] [%] [-]"); [done..|].
     iIntros "Hγσ_s".
-    iApply (sim_tgt_link_left_recv with "[-]").
+    iApply (sim_tgt_link_recv_left with "[-]").
     iApply (sim_tgt_rec_Waiting_raw _ []).
     iSplit; [|by iIntros].
     iIntros (???? Hin) "!>". iIntros (?). simplify_map_eq.
-    iApply (sim_tgt_link_left with "[-]").
-    iMod (heapUR_alloc_blocks _ (h_blocks h) with "Hh") as "[Hh _]". { set_solver. }
+
+    iMod (heapUR_alloc_blocks _ (h_blocks h) with "[$]") as "[Hinv _]". { set_solver. }
     rewrite right_id_L heap_from_blocks_h_blocks.
 
-    iApply (sim_gen_expr_intro _ [] with "[Hh]"). { done. } { by iFrame. }
+    (* Target's spec module (Right linking case - locle) *)
+    iMod (mstate_var_alloc (m_state (spec_trans rec_event unit))) as (γσr_t) "Hγσr_t".
+    (* Target's rec module (Left linking case) *)
+    iMod (mstate_var_alloc (m_state rec_trans)) as (γσl_t) "Hγσl_t".
+    (* call stack of linking module  *)
+    iMod (mstate_var_alloc (list seq_product_case)) as (γq_t) "Hγq_t".
+    (* Linking event to pass around *)
+    iMod (mstate_var_alloc (option rec_ev)) as (γκ_t) "Hγκ_t".
 
-    set (Π := link_tgt_leftP _ _ _ _).
+    iApply (sim_tgt_link_left_constP_run γq_t γσl_t γσr_t γκ_t with "[$] [$] [$] [$] [-]").
+    iIntros "Hγq_t Hγσr_t Hγκ_t".
 
-    iApply (sim_gen_expr_bind _ [ReturnExtCtx _] with "[-]") => /=.
-    iApply (sim_main_full with "[] [] [] [] [] Hγσ_s"). 1-4: by iApply (rec_fn_intro with "[$]").
-    { iIntros "!>". iApply sim_locle2. 1: done. 1: { by iApply (rec_fn_intro with "[$]"). }
-      iIntros (??). iDestruct 1 as (?? ->) "HC" => /=.
-      iIntros (??????). destruct!/=. rewrite bool_decide_false //. rewrite bool_decide_true //.
-      iApply (sim_tgt_link_right_recv with "[-]"). iApply "HC". iSplit!. iIntros (??). iDestruct 1 as (? ->) "HC" => /=.
-      iIntros (?). simplify_eq.
-      iApply (sim_tgt_link_right with "[-]"). iApply "HC". iSplit!.
-      iIntros (??). iDestruct 1 as (?? -> ->) "HC" => /=.
+    iApply (sim_gen_expr_intro _ [] with "[Hinv]"). { done. } { by iFrame. }
+
+    set (Π := tgt_link_left_constP _ _ _ _ _ _).
+    set PL := (λ (σ : m_state (spec_trans rec_event unit)),
+                 γσr_t ⤳ σ ∗ γκ_t ⤳ @None rec_ev ∗ γq_t ⤳ [None : seq_product_case])%I.
+    iDestruct (sim_locle _ Π _ PL (locle_spec, tt) with "[$] [] [$] [//]") as "H".
+    1: by iApply (rec_fn_intro with "[$]").
+    iMod ("H" with "[]") as "[%Pl [HPl [#Hlocle #Hsplitl]]]".
+    {
+      iIntros "!> %% (% & % & % & (Hγσr_t & ? & ?) & -> & HC)".
+      (* REVIEW - How to do this better with done *)
+      iApply (tgt_link_left_constP_run_elim with "[$] [Hγσr_t] [$]"); [done|].
+      iIntros "Hγq_t Hγσl_t Hγσr_t Hγκ_t".
+      iIntros (??????).
+      destruct!/=. rewrite bool_decide_false //. rewrite bool_decide_true //.
+      iApply (sim_tgt_link_right_constP_recv γq_t γσl_t γσr_t γκ_t
+               with "[$] [Hγσl_t] [Hγσr_t] [$] [-]"); [done..|].
+      iIntros "Hγq_t Hγσl_t Hγκ_t".
+
+      iApply "HC". iSplit!.
+      iIntros (??) "[% [-> HC]]".
+      iApply (tgt_link_right_constP_recv_elim with "[Hγq_t] [Hγσl_t] [$] [-]"); [done..|].
+      iIntros "Hγq_t Hγσl_t Hγσr_t Hγκ_t" (?). simplify_eq.
+      iApply (sim_tgt_link_right_constP_run γq_t γσl_t γσr_t γκ_t
+               with "[$] [Hγσl_t] [Hγσr_t] [$] [-]"); [done..|].
+      iIntros "Hγq_t Hγσl_t Hγκ_t".
+
+      iApply "HC" => /=. iSplit!.
+      iIntros (??) "[% [% [-> HC]]]".
+      iApply (tgt_link_right_constP_run_elim with "[Hγq_t] [Hγσl_t] [$] [-]"); [done..|].
+      iIntros "Hγq_t Hγσl_t Hγσr_t Hγκ_t".
       iIntros (??????). destruct!/=.
-      iApply (sim_tgt_link_left_recv with "[-]"). iApply "HC". iSplit!.
-      iIntros (??). iDestruct 1 as (? ->) "HC" => /=.
+      iApply (sim_tgt_link_left_constP_recv γq_t γσl_t γσr_t γκ_t
+               with "[$] [Hγσl_t] [Hγσr_t] [$] [-]"); [done..|].
+      iIntros "Hγq_t Hγσr_t Hγκ_t".
+
+      iApply "HC". iSplit!.
+      iIntros (??) "[% [-> HC]]" => /=.
+      iApply (tgt_link_left_constP_recv_elim with "[Hγq_t] [Hγσr_t] [$] [-]"); [done..|].
+      iIntros "Hγq_t Hγσl_t Hγσr_t Hγκ_t".
       iIntros (?). simplify_eq.
-      iApply (sim_tgt_link_left with "[-]"). by iApply "HC". } { done. }
-    iSplit!.
-    - iIntros "!>" (??). iDestruct 1 as (??? ->) "[Hγσ_s HC]" => /=.
-      iIntros  (??????). destruct!/=. rewrite !bool_decide_false //.
+      iApply (sim_tgt_link_left_constP_run γq_t γσl_t γσr_t γκ_t
+               with "[$] [Hγσl_t] [Hγσr_t] [$] [-]"); [done..|].
+      iIntros "Hγq_t Hγσr_t Hγκ_t".
+
+      iApply "HC". iSplit!. iFrame.
+    }
+
+    iDestruct (mstate_var_merge with "Hγs [$]") as "[_ Hγs]".
+    set PL' := (λ (σ : m_state (spec_trans rec_event unit)), γσ_s ⤳ σ ∗ (∃ σ', PL σ'))%I.
+
+    iDestruct (call_print_sim Hspec _ PL' Π with "[$] [] []") as "#Hprint".
+    1: by iApply (rec_fn_intro with "[$]").
+
+    {
+      iIntros "!> %% (% & % & % & (Hγσ_s & % & Hγσr_t & ? & ?) & -> & HC)".
+      iApply (tgt_link_left_constP_run_elim with "[$] [Hγσr_t] [$]"); [done|].
+      iIntros "Hγq_t Hγσl_t Hγσr_t Hγκ_t".
+      iIntros (??????). destruct!/=. rewrite bool_decide_false //.
       iApply (sim_tgt_constP_elim γσ_t γσ_s γκ with "[Hγσ_s] [-]"); [done..|].
       iIntros "Hγσ_s Hγσ_t Hγκ".
-      iApply "HC". iSplit!. iIntros (??). iDestruct 1 as (->) "HC".
+
+      iApply "HC". iSplit!. iIntros (??) "[-> HC]".
       iApply (sim_src_constP_next with "[Hγσ_t] [Hγκ] [Hγσ_s] [%] [-]"); [done..|].
       iIntros "Hγσ_s".
       iApply (sim_tgt_link_None with "[-]"). iIntros "!>" (??????). destruct!/=.
       iApply (sim_tgt_constP_elim γσ_t γσ_s γκ with "[Hγσ_s] [-]"); [done..|].
       iIntros "Hγσ_s Hγσ_t Hγκ".
-      iApply "HC". iSplit!. iIntros (??) "[% HC]". simplify_eq.
+
+      iApply "HC". iSplit!. iIntros (??) "[-> HC]".
       iApply (sim_src_constP_next with "[Hγσ_t] [Hγκ] [Hγσ_s] [%] [-]"); [done..|].
       iIntros "Hγσ_s". iApply sim_gen_stop.
       iApply (sim_tgt_constP_elim γσ_t γσ_s γκ with "[Hγσ_s] [-]"); [done..|].
       iIntros "Hγσ_s Hγσ_t Hγκ".
-      iApply "HC". iSplit!. iIntros (??). iDestruct 1 as (?? -> ->) "HC".
+
+      iApply "HC". iSplit!. iIntros (??) "(% & % & -> & -> & HC)".
       iApply (sim_src_constP_next with "[Hγσ_t] [Hγκ] [Hγσ_s] [%] [-]"); [done..|].
       iIntros "Hγσ_s". destruct!/=.
-      iApply (sim_tgt_link_left_recv with "[-]").
-      iApply ("HC" with "[-]"). iFrame. iSplit!.
-      iIntros (??). iDestruct 1 as (? ->) "HC".
-      iIntros (?). simplify_eq.
-      iApply (sim_tgt_link_left with "[-]").
-      iApply "HC". iSplit!.
-    - iIntros (?) "[% [Hγσ_s [Hs %]]]". iApply sim_tgt_rec_ReturnExt.
-      iIntros (???) "Hfns''' Hh !>".
-      iIntros (??) "[-> [-> _]]" => /=. iIntros (??????). destruct!/=.
-      iApply (sim_tgt_constP_elim γσ_t γσ_s γκ with "[Hγσ_s] [-]"); [done..|].
-      iIntros "Hγσ_s Hγσ_t Hγκ".
-      iApply "Hs".
-  Qed.
+      iApply (sim_tgt_link_left_constP_recv γq_t γσl_t γσr_t γκ_t
+               with "[$] [Hγσl_t] [Hγσr_t] [$] [-]"); [done..|].
+      iIntros "Hγq_t Hγσr_t Hγκ_t".
 
-End memmove.
+      iApply ("HC" with "[-]"). iFrame. iSplit!.
+      iIntros (??) "[% [-> HC]]".
+      iApply (tgt_link_left_constP_recv_elim with "[Hγq_t] [Hγσr_t] [$] [-]"); [done..|].
+      iIntros "Hγq_t Hγσl_t Hγσr_t Hγκ_t %". simplify_eq.
+      iApply (sim_tgt_link_left_constP_run γq_t γσl_t γσr_t γκ_t
+               with "[$] [Hγσl_t] [Hγσr_t] [$] [-]"). 1-2: done.
+      iIntros "???".
+
+      iApply "HC". iSplit!. iFrame.
+    }
+
+    iApply (sim_gen_expr_bind _ [ReturnExtCtx _] with "[-]") => /=.
+    iApply (sim_main with "[] [] [] [$]"). 1-3: by iApply (rec_fn_intro with "[$]").
+    iFrame. iSplit!.
+    iIntros (??) "[? [-> HΦ]]".
+
+    iDestruct ("Hsplitl" $! tt with "[$]") as "[%σ' [HPL ?]]".
+
+    iApply "Hprint". iFrame. iSplit!;[done|]. iIntros (?) "[% [? [? %]]]".
+    iApply "HΦ".
+    iIntros (??) "[? HΦ]".
+    iApply "Hprint".
+    iFrame. iSplit!;[done|].
+    iIntros (?) "[%σ_s' [[Hγσ_s [% [Hγσr_t [Hγκ_t Hγq_t]]]] [? %]]]".
+    iApply "HΦ".
+    iIntros (?->).
+    iApply (sim_gen_expr_bind _ [ReturnExtCtx _] with "[-]").
+
+    iApply (sim_gen_expr_stop). iSplit!. iFrame.
+
+    iApply sim_gen_expr_None. iIntros (??) "?? %% /= [-> [-> ?]]".
+    iApply (tgt_link_left_constP_run_elim with "Hγq_t [Hγσr_t] [$]");[done|].
+    iIntros "Hγq_t Hγσl_t Hγσr_t Hγκ_t".
+    iApply (sim_tgt_constP_elim γσ_t γσ_s γκ with "[Hγσ_s] [-]"); [done..|].
+    iIntros "Hγσ_s Hγσ_t Hγκ".
+
+    iMod (mstate_var_split γs_s () with "[$]") as "[Hγs_s Hγs_s']".
+    (* TODO *)
+    iApply (sim_gen_expr_intro _ tt with "[Hγs_s]") => //=.
+    { destruct σ_s'. simpl. destruct u. done. }
+    iApply sim_src_TUb_end.
+Qed.
+
+End main.
 
 Lemma memmove_refines_spec :
   trefines (rec_link {["main"; "memmove"; "memcpy"]} {["locle"]}
